Graph.v
@@ -18,108 +18,407 @@ Module Graph.
 
   (** Graph **)
 
-  Class Graph (L : Type) (edge : L -> L -> Prop) : Type :=
-    {
-      L_dec : EqDec L eq where "p --> q" := (edge p q);
-      edge_dec : forall p q, {p --> q} + {~ p --> q}(*;
-      root_no_pred : forall p:L, ~ edge p root*)
-    }.
+  (* bool or prop ?
 
-  Generalizable Variables L root edge.
+pro bool:
+-eine Funktion repräsentiert den Graph
+-Beweise in Richtung bool -> Prop trivial
+-in andere Richtung Entscheidbarkeitsbeweise notwendig (benutze library) 
+  (^ geht das ? nicht alles endl.)
 
-  Notation "p --> q" := ((fun (L : Type) (edge : L -> L -> Prop) (_ : Graph L edge) => edge) _ _ _ p q)
-                          (at level 55, right associativity).
+contra: 
+-kann in logischen Ausdrücken nicht direkt verwendet werden
+-Graphen können einfacher formuliert werden
+(-stauts quo)
 
-(*  Infix "-->" := edge (at level 55, right associativity).*)
-
-  Definition in_graph `{Graph} (p : L) := exists q, p --> q \/ q --> p.
+   *)
   
-  Inductive Path `{Graph} : L -> L -> ne_list L -> Prop :=
-  | PathSingle a : Path a a (ne_single a)
-  | PathCons {a b c π} : Path a b π -> b --> c -> Path a c (c :<: π).
 
-  Definition Dom `{Graph} r p q := forall π, Path r q π -> In p π.
+  Ltac destructH' H :=
+    lazymatch type of H with
+    | ?P /\ ?Q => let H1 := fresh H in
+                let H2 := fresh H in
+                destruct H as [H1 H2]; destructH' H1; destructH' H2
+    | exists x, ?P => let x0 := fresh x in
+                destruct H as [x0 H]; destructH' H
+    | _ => idtac
+    end.
 
-  Program Instance sub_Graph `{G : Graph} (l : list L)
-    : Graph L (fun p q => (p ∈ l /\ q ∈ l /\ edge p q)).
-  Next Obligation. apply L_dec. Qed.
-  Next Obligation.
-    destruct (edge_dec p q).
-    destruct (in_dec L_dec p l).
-    destruct (in_dec L_dec q l).
-    1: left; firstorder. all: right; firstorder.
-  Qed.
-  
-  Program Instance union_Graph
-          {L : Type} {edge1 edge2 : L -> L -> Prop}
-          (G1 : Graph L edge1) (G2 : Graph L edge2)
-    : Graph L (fun p q => edge1 p q \/ edge2 p q).
-  Next Obligation. apply L_dec. Qed.
-  Next Obligation.
-    destruct (@edge_dec _ edge1 _ p q), (@edge_dec _ edge2 _ p q); tauto.
-  Qed.
-  (*Next Obligation.
-    intro H. destruct H; apply root_no_pred in H; contradiction.
-  Qed.*)
+  Ltac destructH :=
+    match goal with
+    | [H : ?P /\ ?Q |- _ ] => let H1 := fresh H in
+                         let H2 := fresh H in
+                         destruct H as [H1 H2]; destructH' H1; destructH' H2
+    | [H : exists x, ?P |- _ ] => let x0 := fresh x in
+                           destruct H as [x0 H]; destructH' H
+    end.
 
-  Program Instance minus_Graph
-          {L : Type} {edge1 edge2 : L -> L -> Prop}
-          (G1 : Graph L edge1) (G2 : Graph L edge2)
-    : Graph L (fun p q => edge1 p q /\ ~ edge2 p q).
-  Next Obligation. apply L_dec. Qed.
-  Next Obligation.
-    destruct (@edge_dec _ edge1 _ p q), (@edge_dec _ edge2 _ p q); tauto.
-  Qed. (*
-  Next Obligation.
-    intro H. destruct H; apply root_no_pred in H; contradiction.
-  Qed.*)
+  Section Graph.
+    
+    Variable L : Type.
+    Variables edge edge1 edge2 : L -> L -> bool.
+    
+    Hypothesis L_dec : EqDec L eq.
 
-  Lemma path_front `{Graph} p q π :
-    Path p q π -> ne_front π = q.
-  Admitted.
-  
-  Lemma path_back `{Graph} p q π :
-    Path p q π -> ne_front π = p.
-  Admitted.
+    Local Notation "p -->b q" := (edge p q) (at level 55, right associativity).
+    Local Notation "p --> q" := (p -->b q = true) (at level 55, right associativity).
+    
+    Inductive Path : L -> L -> ne_list L -> Prop :=
+    | PathSingle a : Path a a (ne_single a)
+    | PathCons {a b c π} : Path a b π -> b --> c -> Path a c (c :<: π).
 
-  Lemma postfix_path `{Graph} l p q q' l' :
-    Path q' q l'
-    -> Postfix (l :r: p) l'
-    -> Path p q (nl_rcons l p).
-  Admitted.
+    Local Notation "p -->* q" := (exists π, Path p q π) (at level 55).
 
-  Definition Path' `{Graph} π := Path (ne_back π) (ne_front π) π.
+    Definition Dom r p q := forall π, Path r q π -> p ∈ π.
+
+    Lemma dominant_root r p : Dom r r p.
+    Proof.
+      intros π Hpath. induction Hpath;cbn;eauto.
+    Qed.
+
+    Lemma dominant_self p q : Dom p q q.
+    Proof.
+      intros π Hπ. induction Hπ;cbn;eauto.
+    Qed.
+    
+    Lemma path_front p q π :
+      Path p q π -> ne_front π = q.
+    Proof.
+      intro H. induction H; cbn; eauto.
+    Qed.
+    
+    Lemma path_back p q π :
+      Path p q π -> ne_back π = p.
+    Proof.
+      intro H. induction H; cbn; eauto.
+    Qed.
+
+    Lemma path_dec p q π :
+      {Path p q π} + {~ Path p q π}.
+    Proof.
+      revert q; induction π; intros q.
+      - decide' (p == a); decide' (q == p). 1: left; econstructor.
+        all: right; intro N; inversion N; firstorder.
+      - decide' (q == a);
+          [destruct (edge (ne_front π) q) eqn:E;
+           [destruct (IHπ (ne_front π))|]|].
+        1: left; econstructor; eauto.
+        all: right; intro N; inversion N;subst. 3: eapply c; reflexivity.
+        all: eapply path_front in H0 as H0'; subst b. 1:contradiction.
+        rewrite <-not_true_iff_false in E. contradiction.
+    Qed.
+
+    Lemma path_app π ϕ p q r : Path p q π -> Path q r ϕ -> Path p r (ϕ :+ tl π).
+    Admitted.
+
+    (* this is not used : { *)
+    Inductive uniqueIn {A : Type} (a : A) : list A -> Prop := 
+    | UniqueIn (l : list A) : a ∉ l -> uniqueIn a (a :: l)
+    | UniqueCons (b : A) (l : list A) : uniqueIn a l -> a <> b -> uniqueIn a (b :: l).
+
+    Lemma uniqueIn_app {A : Type} `{EqDec A eq} (a : A) l1 l2
+      : uniqueIn a l1 -> a ∉ l2 -> uniqueIn a (l1 ++ l2).
+    Proof.
+      intros Huq Hin.
+      induction l1; cbn; eauto.
+      - inversion Huq.
+      - decide' (a == a0).
+        + econstructor; eauto. inversion Huq; eauto. intro N. eapply in_app_or in N. firstorder.
+        + econstructor 2; eauto. eapply IHl1. inversion Huq; [contradiction|eauto].
+    Qed.
+    
+    Lemma path_glue_loop p r (π0 π1 : ne_list L) :
+      Path p r π0
+      -> uniqueIn r π0 -> uniqueIn r π1
+      -> uniqueIn r (π1 ++ tl π0).
+    Proof.
+      intros Hpr Huq0 Huq1.
+      eapply uniqueIn_app; eauto.
+      induction π0; cbn; eauto.
+      clear - Huq0 Hpr. eapply path_front in Hpr. cbn in *. subst a. intro N.
+      inversion Huq0; eauto.
+    Qed.
+
+    Lemma uniqueIn_NoDup {A : Type} `{EqDec A eq} (l : list A)
+      : NoDup l <-> forall a, a ∈ l -> uniqueIn a l.
+    Proof.
+      rename H into Hed.
+      split; [intros Hnd a Hin|intros H].
+      - induction l; inversion Hin; inversion Hnd; cbn; subst.
+        + econstructor; eauto.
+        + exploit IHl. econstructor;eauto. intro N. subst. contradiction.
+      - induction l; econstructor.
+        + specialize (H a (or_introl (eq_refl))). inversion H; eauto.
+        + eapply IHl. intros b Hb.
+          specialize (H b (or_intror Hb)).
+          decide' (a == b); inversion H; eauto; subst; contradiction.
+    Qed.
+    (* } *)
+
+    Lemma prefix_single {A : Type} (a : A) (l : ne_list A)
+      : Prefix (ne_single a) l -> ne_back l = a.
+    Proof.
+      intro H. induction l; inversion H; cbn; eauto; subst. inversion H2.
+      destruct l; cbn in *; congruence.
+    Qed.
+
+    Lemma path_prefix_path p q (π ϕ : ne_list L) : Path p q π -> Prefix ϕ π -> Path p (ne_front ϕ) ϕ.
+    Proof.
+      intros Hpq Hpre. revert dependent q. dependent induction Hpre; intros q Hpq.
+      - eapply ne_to_list_inj in x. subst. erewrite path_front; eauto.
+      - destruct π.
+        + inversion x. subst l'. inversion Hpre; subst. destruct ϕ; cbn in H2; congruence.
+        + rewrite nlcons_to_list in x. eapply ne_to_list_inj in x.
+          eapply IHHpre; cycle 1.
+          * instantiate (1:=π). destruct l';[cbn in x;congruence|].
+            cbn in x. inversion x. simpl_nl. reflexivity.
+          * instantiate (1:= ne_front π). inversion Hpq; subst. erewrite path_front; eauto.
+          * reflexivity.
+    Qed.
+    
+    Lemma path_postfix_path p q (π ϕ : ne_list L) : Path p q π -> Postfix ϕ π -> Path (ne_back ϕ) q ϕ.
+    Proof.
+    Admitted.
+
+    Definition prefix_incl : forall (A : Type) (l l' : list A), Prefix l l' -> l ⊆ l'
+      := fun (A : Type) (l l' : list A) (post : Prefix l l') =>
+           Prefix_ind A (fun l0 l'0 : list A => l0 ⊆ l'0) (fun l0 : list A => incl_refl l0)
+                      (fun (a : A) (l0 l'0 : list A) (_ : Prefix l0 l'0) (IHpost : l0 ⊆ l'0) =>
+                         incl_appr (a :: nil) IHpost) l l' post.      
+
+    Lemma prefix_NoDup {A : Type} (l l' : list A) : Prefix l l' -> NoDup l' -> NoDup l.
+    Proof.
+      intros Hpre Hnd. induction Hpre; eauto.
+      inversion Hnd; subst; eauto.
+    Qed.
+    
+    Lemma path_NoDup p q : p -->* q -> exists π, Path p q π /\ NoDup π.
+    Proof.
+      intros [ϕ Hto].
+      induction Hto.
+      - exists (ne_single a). split;econstructor;eauto. econstructor.
+      - destruct IHHto as [ψ [IHHto IHnodup]].
+        destruct (In_dec c ψ).
+        + eapply prefix_nincl_prefix in H0.
+          exists (c :< prefix_nincl c ψ). split.
+          * rewrite nlcons_to_list in H0.
+            eapply path_prefix_path in H0; eauto; cbn in *; simpl_nl' H0; eauto.
+          * eapply prefix_NoDup; eauto. simpl_nl; eauto.
+        + exists (c :<: ψ). split;econstructor;eauto.
+    Qed.
+
+    Lemma in_nlcons {A : Type} `{EqDec A eq} (l : list A) (a b : A)
+      : a ∈ (b :< l) <-> a = b \/ a ∈ l.
+    Proof.
+      split; intro Q.
+      - revert dependent b. induction l; cbn in *;intros b Q;[firstorder|].
+        destruct Q;[firstorder|].
+        right. specialize (IHl a0 H0). firstorder.
+      - revert dependent b. induction l; cbn in *;intros b Q;[firstorder|].
+        destruct Q;[firstorder|].
+        right. eapply IHl. firstorder.
+    Qed.
+
+    Lemma in_ne_conc {A : Type} `{EqDec A eq} (l l' : ne_list A)
+      : forall a, a ∈ (l :+: l') <-> a ∈ l \/ a ∈ l'.
+    Proof.
+      split; revert a; induction l;intros b Q; cbn in *; firstorder 0.
+    Qed.
+
+    Lemma in_nl_conc {A : Type} `{EqDec A eq} (l : ne_list A) l' (a : A)
+      : a ∈ (l :+ l') <-> a ∈ l \/ a ∈ l'.
+    Proof.
+      split;revert a;induction l'; intros b Q; cbn in *; [firstorder| |firstorder|].
+      - eapply in_ne_conc in Q. repeat destruct Q; eauto. eapply in_nlcons in H0. destruct H0;eauto.
+      - eapply in_ne_conc. repeat destruct Q; eauto. right. eapply in_nlcons. firstorder.
+    Qed.
 
 
-  Lemma ne_to_list_not_nil {A:Type} (l : ne_list A) :
-    nil <> l.
-  Proof.
-    intro N. induction l; cbn in *; congruence.
-  Qed.
-  
-  Lemma postfix_front {A : Type} (l l' : ne_list A) :
-    Postfix l l'
-    -> ne_front l = ne_front l'.
-  Proof.
-    intros H. dependent induction H.
-    - apply ne_to_list_inj in x; rewrite x; eauto.
-    - rewrite rcons_nl_rcons in x. apply ne_to_list_inj in x. 
-      rewrite <-x. destruct l'0.
-      + exfalso. inversion H; [eapply ne_to_list_not_nil|eapply rcons_not_nil]; eauto.
-      + cbn. erewrite IHPostfix; eauto; [|rewrite nlcons_to_list; reflexivity]. simpl_nl; reflexivity.
-  Qed.
-  
-  Lemma path_postfix_path `{Graph} p q q' (l l' : ne_list L) :
-    Path p q l
-    -> Postfix l' l
-    -> Path p q' l'.
-  Proof.
-  Admitted. (*
+    Lemma path_to_elem p q r π : Path p q π -> r ∈ π -> exists ϕ, Path p r ϕ /\ Prefix ϕ π.
+    Proof.
+      revert dependent q.
+      induction π; intros q Hpath Hin; cbn in *; eauto.
+      - destruct Hin;[subst|contradiction].
+        eapply path_front in Hpath as Hfront. eapply path_back in Hpath as Hback. subst p q; cbn in *.
+        eexists; split; eauto. econstructor.
+      - destruct Hin.
+        + subst a. eapply path_back in Hpath as Hback. eapply path_front in Hpath as Hfront.
+          subst p q; cbn in *. exists (r :<: π); split; eauto.
+          econstructor.
+        + inversion Hpath; subst. specialize (IHπ b H4 H) as [ϕ [Hϕ Hpre]].
+          eexists;split;eauto. econstructor;eauto.
+    Qed.
+
+    Lemma path_from_elem p q r π : Path p q π -> r ∈ π -> exists ϕ, Path r q ϕ /\ Postfix ϕ π.
+    Proof.
+      intros Hpath Hin. exists (postfix_nincl r π >: r).
+      assert (Postfix (postfix_nincl r π >: r) π) as H;[|split];eauto.
+      - simpl_nl. eapply postfix_nincl_spec; eauto.
+      - eapply path_postfix_path in Hpath;eauto. simpl_nl' Hpath;eauto.
+    Qed.        
+    
+    Lemma dom_nin r p q π : Dom r p q -> Path r p π -> NoDup π -> q ∈ π -> p = q.
+    Proof.
+      intros Hdom Hpath Hnd Hin. eapply path_to_elem in Hpath as Hpath';eauto.
+      destruct Hpath' as [ϕ [Hϕ Hpre]].
+      inversion Hpre; subst.
+      - eapply ne_to_list_inj in H1. subst. eapply path_front in Hpath. eapply path_front in Hϕ.
+        subst p q; eauto.
+      - exfalso.
+        rewrite nlcons_to_list in H. eapply ne_to_list_inj in H; subst π.
+        eapply path_front in Hpath. cbn in Hpath. simpl_nl' Hpath. subst a.
+        eapply Hdom in Hϕ as Hϕ'. eapply prefix_incl in H1. eapply H1 in Hϕ'.
+        simpl_nl' Hnd. inversion Hnd; subst; contradiction.
+    Qed.
+    
+    Lemma in_ne_back {A : Type} `{EqDec A eq} (l : ne_list A) : ne_back l ∈ l.
+    Proof.
+      induction l; cbn; eauto.
+    Qed.
+    
+    Lemma dom_trans r h p q : r -->* h -> Dom r h p -> Dom r p q -> Dom h p q.
+    Proof.
+      intros Hϕ Hdom_h Hdom_p π Hπ.
+      eapply path_NoDup in Hϕ as [ϕ [Hϕ Hndup]].
+      eapply path_app in Hπ as Hπ';eauto. eapply Hdom_p in Hπ'.
+      eapply in_nl_conc in Hπ'.
+      destruct Hπ'; eauto.
+      enough (h = p).
+      - subst h. eapply path_back in Hπ. subst p; eapply in_ne_back.
+      - eapply dom_nin. 3: eassumption. 1: apply Hdom_h. 1: eauto.
+        destruct ϕ; cbn in H; [contradiction|]. right; eauto.
+    Qed.
+    
+    Definition intersection_edge := fun p q => edge1 p q && edge2 p q.
+
+    Definition union_edge := fun p q => edge1 p q || edge2 p q.
+
+    Definition minus_edge := fun p q => edge1 p q && negb(edge2 p q).
+
+    Definition sub_graph := forall p q, edge1 p q = true -> edge2 p q = true.
+
+    Definition acyclic := forall p q, p --> q -> ~ p -->* q.
+
+    Lemma postfix_path l p q q' l' :
+      Path q' q l'
+      -> Postfix (l :r: p) l'
+      -> Path p q (nl_rcons l p).
+    Admitted.
+
+    Definition Path' π := Path (ne_back π) (ne_front π) π.
+
+
+    Lemma ne_to_list_not_nil {A:Type} (l : ne_list A) :
+      nil <> l.
+    Proof.
+      intro N. induction l; cbn in *; congruence.
+    Qed.
+    
+    Lemma postfix_front {A : Type} (l l' : ne_list A) :
+      Postfix l l'
+      -> ne_front l = ne_front l'.
+    Proof.
+      intros H. dependent induction H.
+      - apply ne_to_list_inj in x; rewrite x; eauto.
+      - rewrite rcons_nl_rcons in x. apply ne_to_list_inj in x. 
+        rewrite <-x. destruct l'0.
+        + exfalso. inversion H; [eapply ne_to_list_not_nil|eapply rcons_not_nil]; eauto.
+        + cbn. erewrite IHPostfix; eauto; [|rewrite nlcons_to_list; reflexivity].
+          simpl_nl; reflexivity.
+    Qed.
+
+  (*
+    Lemma path_postfix_path p q q' (l l' : ne_list L) :
+      Path p q l
+      -> Postfix l' l
+      -> Path p q' l'.
+    Proof.
+    Admitted. 
     intros Hpath Hpost. dependent induction Hpost.
     - apply ne_to_list_inj in x. setoid_rewrite x; eauto.
     - unfold Path'. specialize (IHHpost H). erewrite postfix_front; eauto.
   Qed.*)
 
+  End Graph.
+
+  Arguments Path {L}.
+  Arguments Dom {L}.
+  Arguments intersection_edge {L}.
+  Infix "∩" := intersection_edge (at level 50).
+  Arguments union_edge {L}.
+  Infix "∪" := union_edge (at level 51).
+  Arguments minus_edge {L}.
+  Infix "∖" := minus_edge (at level 49).
+  Arguments sub_graph {L}.
+  Arguments acyclic {L}.
+  
+  Lemma subgraph_path {L : Type} (edge1 edge2 : L -> L -> bool) p q :
+    sub_graph edge1 edge2 -> (exists π, Path edge1 p q π) -> (exists ϕ, Path edge2 p q ϕ).
+  Proof.
+    intros Hsub [π Hpath]. unfold sub_graph in Hsub. induction Hpath.
+    - exists (ne_single a). econstructor.
+    - destruct IHHpath as [ϕ IHHpath]. exists (c :<: ϕ). econstructor; eauto.
+  Qed.
+
+  Lemma subgraph_path' {L : Type} (edge1 edge2 : L -> L -> bool) p q π :
+    sub_graph edge1 edge2 -> Path edge1 p q π -> Path edge2 p q π.
+  Proof.
+    intros Hsub Hpath. unfold sub_graph in Hsub. induction Hpath.
+    - econstructor.
+    - econstructor; eauto. 
+  Qed.
+  
+  Lemma acyclic_subgraph_acyclic {L : Type} (edge1 edge2 : L -> L -> bool) :
+    sub_graph edge1 edge2 -> acyclic edge2 -> acyclic edge1.
+  Proof.
+    intros Hsub Hacy p q Hedge N. unfold acyclic, sub_graph in *. 
+    eapply Hacy; eauto. destruct N as [π Hpath].
+    eapply subgraph_path; eauto.
+  Qed.
+
+  Lemma minus_subgraph {L : Type} (edge1 edge2 : L -> L -> bool) :
+    sub_graph (edge1 ∖ edge2) edge1.
+  Proof.
+    intros p q Hsub. unfold minus_edge in Hsub. conv_bool. firstorder.
+  Qed.
+
+  Lemma intersection_subgraph1 {L : Type} (edge1 edge2 : L -> L -> bool) :
+    sub_graph (edge1 ∩ edge2) edge1.
+  Proof.
+    intros p q Hinter. unfold intersection_edge in Hinter. conv_bool. firstorder.
+  Qed.
+  
+  Lemma intersection_subgraph2 {L : Type} (edge1 edge2 : L -> L -> bool) :
+    sub_graph (edge1 ∩ edge2) edge2.
+  Proof.
+    intros p q Hinter. unfold intersection_edge in Hinter. conv_bool. firstorder.
+  Qed.
+
+  Lemma intersection2_subgraph {L : Type} (edge edge1 edge2 : L -> L -> bool) :
+    sub_graph edge1 edge2
+    -> sub_graph (edge1 ∩ edge) (edge2 ∩ edge).
+  Proof.
+    intros Hsub p q Hinter. unfold intersection_edge in *. unfold sub_graph in Hsub.
+    conv_bool. destruct Hinter as [Hinter1 Hinter2]. eapply Hsub in Hinter1.
+    rewrite Hinter1,Hinter2; cbn;eauto.
+  Qed.
+
+  Lemma union_subgraph {L : Type} (edge1 edge1' edge2 edge2' : L -> L -> bool) :
+    sub_graph edge1 edge1' -> sub_graph edge2 edge2' -> sub_graph (edge1 ∪ edge2) (edge1' ∪ edge2').
+  Proof.
+    intros Hsub1 Hsub2 p q Hu. unfold union_edge, sub_graph in *.
+    conv_bool. destruct Hu as [Hu|Hu];firstorder 1.
+  Qed.    
+  
+  Lemma dom_intersection {L : Type} (edge1 edge2 : L -> L -> bool) r p q :
+    Dom edge1 r p q -> Dom (edge1 ∩ edge2) r p q.
+  Proof.
+    intros Hdom.
+    unfold Dom in *. intros. apply Hdom.
+    eapply subgraph_path';eauto.
+    eapply intersection_subgraph1.
+  Qed.
+    
 End Graph.
 (*+ CFG +*)
 
@@ -128,83 +427,116 @@ Module CFG.
   Export Graph.
   
   (** basic parameters **)
-  Parameter Lab : Type.  
+  Parameter Lab : Type.
   Parameter all_lab : list Lab.
   Parameter all_lab_spec : forall l, l ∈ all_lab.
   Parameter Lab_dec : EqDec Lab eq.
+
+  Hint Resolve Lab_dec.
      
-  Program Instance Lab_Graph
-          (rel : Lab -> Lab -> Prop)
-          (rel_dec : forall a b, {rel a b} + {~ rel a b})
-    : Graph Lab rel.
+(*  Notation "p '-->*' q" := (exists π, Path p q π) (at level 55, right associativity).*)
 
-  Notation "p '-->*' q" := (exists π, Path p q π) (at level 55, right associativity).
-
-  Reserved Notation "p -a> q" (at level 55).
-  Reserved Notation "p -a>* q" (at level 55).
+  Reserved Infix "-->b" (at level 55).
+  Reserved Infix "-a>" (at level 55).
+  Reserved Infix "-a>*" (at level 55).
 
   Definition decidableT (a : Prop) := {a} + {~ a}.
 
-  Definition minus_edge (rel_sub rel_min : Lab -> Lab -> Prop) : Lab -> Lab -> Prop :=
-    (fun p q : Lab => rel_sub p q /\ ~ rel_min p q).
 
-  Lemma minus_dec (rel_sub rel_min : Lab -> Lab -> Prop) :
+(*  Lemma minus_dec (rel_sub rel_min : Lab -> Lab -> Prop) :
     (forall p q, decidableT (rel_sub p q))
     -> (forall p q, decidableT (rel_min p q))
     -> (forall p q, decidableT (minus_edge rel_sub rel_min p q)).
   Proof.
     unfold decidableT, minus_edge. intros sdec mdec.
     intros. specialize (sdec p q). specialize (mdec p q). destruct sdec, mdec; firstorder.
-  Qed.
+  Qed.*)
+
   
-  Class redCFG (edge : Lab -> Lab -> Prop) (G : Graph Lab edge) (root : Lab)
-        {acyclic_edge : Lab -> Lab -> Prop}
-        (acyclic_fragment : Graph Lab acyclic_edge) :=
-    {
-      loop_head_dom : forall ql qh, minus_edge edge acyclic_edge ql qh -> @Dom _ _ G root qh ql
-                   where "p -a> q" := (acyclic_edge p q);
-      acyclic_edge_incl : forall p q, p -a> q -> p --> q 
-                   where "p '-a>*' q" := (exists π, @Path _ acyclic_edge acyclic_fragment p q π);
-      (*reach_acy : forall (p : Lab), root -a>* p; this is too much, we want to allow incomplete graphs*)
-      acyclic : forall (p q : Lab), p -a> q -> ~ q -a>* p;
-    }.
-
-  Notation "p '-a>' q" := ((fun (acyclic_edge : Lab -> Lab -> Prop)
-                              (acyclic_fragment : Graph Lab acyclic_edge)
-                              (_ : redCFG _ _ acyclic_fragment) => acyclic_edge) _ _ _ p q)
-                            (at level 55).
   
-  Definition AcyPath `{redCFG} : Lab -> Lab -> ne_list Lab -> Prop :=
-    @Path _ _ acyclic_fragment.
+  Class redCFG (edge : Lab -> Lab -> bool) (root : Lab) 
+        (a_edge : Lab -> Lab -> bool)
+    :=
+      {
+        back_edge_b := minus_edge edge a_edge
+                       where "p -->b q" := (edge p q);
+                       
+        back_edge := (fun p q => back_edge_b p q = true)
+                     where "p --> q"  := (p -->b q = true);
+        loop_head_dom : forall ql qh, back_edge ql qh -> Dom edge root qh ql
+        where "p -a> q" := (a_edge p q = true);
+        a_edge_incl : sub_graph a_edge edge
+        where "p '-a>*' q" := (exists π, Path a_edge p q π);
+        a_edge_acyclic : acyclic a_edge;
+        in_graph p := exists q, p --> q \/ q --> p;
+        reachability : forall q, in_graph q -> (exists π, Path edge root q π)
+      }.
+  
+  Notation "p '-a>b' q" := ((fun (a_edge : Lab -> Lab -> bool)
+                              (_ : redCFG _ _ a_edge) => a_edge) _ _ p q)
+                             (at level 55).
+  
+  Notation "p '-a>' q" := (p -a>b q = true) (at level 55).
 
-  Notation "p '-a>*' q" := (exists π, AcyPath p q π) (at level 55).
+  Infix "-->b" := ((fun (edge : Lab -> Lab -> bool)
+                      (_ : redCFG edge _ _) => edge)_ _) (at level 55).
 
-  Generalizable Variables G root acyclic_edge acyclic_fragment edge.
+  Notation "p --> q" := (p -->b q = true) (at level 55, right associativity).
 
-  Definition back_edge {edge acyclic_edge : Lab -> Lab -> Prop}
-             {acyclic_fragment : Graph Lab acyclic_edge}
+  Notation "p '-->*' q" := ((fun (edge : Lab -> Lab -> bool)
+                              (_ : redCFG edge _ _) => exists π, Path edge p q π) _ _)
+                             (at level 55, right associativity).
+
+  Notation "p '-a>*' q" := ((fun (a_edge : Lab -> Lab -> bool)
+                               (_ : redCFG _ _ a_edge)
+                             => exists π, Path a_edge p q π) _ _) (at level 55).
+
+  Generalizable Variables edge root a_edge.
+  
+  Definition CPath `{redCFG} := Path edge.
+
+  Definition CPath' `{redCFG} π := CPath (ne_front π) (ne_back π) π.
+
+(*  Definition back_edge {edge a_edge : Lab -> Lab -> Prop}
              {G : Graph Lab edge} {root : Lab}
-             {_ : @redCFG edge _ root _ acyclic_fragment} := minus_edge edge acyclic_edge.
+             {_ : @redCFG edge G root a_edge} := minus_edge edge a_edge.*)
 
   Infix "↪" := back_edge (at level 55).
   
-  Definition loop_head `{H : redCFG} p : Prop :=
+  Definition loop_head `{redCFG} p : Prop :=
     exists q, q ↪ p.
-
-  Lemma loop_head_dec `{H : redCFG} p : decidableT (loop_head p).
-  Admitted.
   
-  Definition loop_contains `{redCFG} qh q : Prop :=
-    exists p, Dom root qh q /\ q -a>* p /\ p --> qh /\ back_edge p qh.
+  Lemma loop_head_dec `{redCFG} p : decidableT (loop_head p).
+  Admitted.
+
+  (* TODO: fix this definition! *)
+  Definition loop_contains `{redCFG} (qh q : Lab) : Prop :=
+    (*qh -->* q /\ *) exists p π, p ↪ qh /\ CPath q p π /\ (qh ∉ π \/ q = qh).
+  (* exists p, Dom edge root qh q /\ q -a>* p /\ p ↪ qh. (old def) *)  
 
   Lemma loop_contains_dec `{redCFG} qh q : {loop_contains qh q} + {~ loop_contains qh q}.
   Admitted.
 
-  Definition loop_contains_b `{redCFG} qh q :=
-    if loop_contains_dec qh q then true else false.
+  Infix "∘" := Basics.compose (at level 40).
+  
+  Definition loop_contains_b `{redCFG} qh q := to_bool (loop_contains_dec qh q).
+
+  Definition deq_loop `{redCFG} q p : Prop :=
+    forall h, loop_contains h p -> loop_contains h q.
+
+  Definition deq_loop_dec `{redCFG} h p : {deq_loop h p} + {~ deq_loop h p}.
+  Admitted.
+
+  Definition deq_loop_b `{redCFG} h p
+    := to_bool (deq_loop_dec h p).
 
   Definition exit_edge `{redCFG} (h p q : Lab) : Prop :=
     loop_contains h p /\ ~ loop_contains h q /\ p --> q.
+
+  Parameter exit_edge_b : forall `{redCFG}, Lab -> Lab -> Lab -> bool.
+  Parameter exit_edge_b_spec : forall `{redCFG} h p q, exit_edge_b h p q = true <-> exit_edge h p q.
+
+  Parameter exit_edge_num : forall `{redCFG}, Lab -> Lab -> nat.
 
   Definition exiting `{redCFG} (h p : Lab) : Prop :=
     exists q, exit_edge h p q.
@@ -215,100 +547,334 @@ Module CFG.
   Fixpoint preds' `{redCFG} (l : list Lab) (p : Lab) : list Lab :=
     match l with
     | nil => nil
-    | q :: l => if (edge_dec p q) then q :: (preds' l p) else preds' l p
+    | q :: l => if (edge q p) then q :: (preds' l p) else preds' l p
     end.
 
   Definition preds `{redCFG} : Lab -> list Lab := preds' all_lab.
 
-  Program Instance loop_CFG `(G : redCFG) (h : Lab) (H : loop_head h) 
-    : @redCFG _ (sub_Graph (filter (loop_contains_b h) all_lab)) h.
+  Definition filter_loop `{redCFG} h := filter (loop_contains_b h) all_lab.
+
+  Definition In_b {A : Type} `{H : EqDec A eq} (a : A) (l : list A)
+    := if in_dec H a l then true else false.
+
+  Lemma loop_contains_loop_head `{redCFG} (qh q : Lab)
+    : loop_contains qh q -> loop_head qh.
+  Proof.
+    intro Q. unfold loop_head, loop_contains in *. destruct Q as [p [_ [Q _]]].
+    eexists; eauto.
+  Qed.
+  
+  Lemma back_edge_incl `{redCFG} p q : back_edge p q -> p --> q.
+  Proof.
+    unfold back_edge,back_edge_b. eapply minus_subgraph.
+  Qed.
+
+  Lemma back_edge_dec `{redCFG} p q : {p ↪ q} + {~ p ↪ q}.
+  Proof.
+    unfold back_edge, back_edge_b, minus_edge.
+    destruct (edge p q), (a_edge p q);cbn;firstorder.
+  Qed.
+
+  Hint Resolve back_edge_dec.
+  
+  Lemma loop_reachs_member `{redCFG} (h q : Lab)
+    : loop_contains h q -> h -->* q.
+  Proof.
+    intros Hloop. unfold loop_contains in Hloop.
+    destructH.
+    assert (in_graph q).
+    {
+      decide' (p == q).
+      - eexists;left;apply back_edge_incl;eauto.
+      - admit.
+    }
+    destruct Hloop3;[|subst q; eexists; econstructor].
+    eapply reachability in H0. destructH. eapply loop_head_dom in Hloop0.
+    eapply path_app in Hloop2;eauto. eapply Hloop0 in Hloop2. eapply in_nl_conc in Hloop2.
+    destruct Hloop2;[contradiction|].
+    assert (h ∈ π0).
+    { destruct π0; cbn in *;[contradiction|right;eauto]. }
+    eapply path_from_elem in H3;eauto. firstorder.
+  Admitted.
+  
+  Lemma dom_loop `{redCFG} h
+    : forall q: Lab, loop_contains h q -> Dom edge root h q.
+  Proof.
+    intros q Hq. unfold loop_contains,CPath in *. intros π Hπ.
+    destructH. eapply path_app in Hq2; eauto.
+    eapply loop_head_dom in Hq2;eauto. eapply in_nl_conc in Hq2.
+    destruct Hq3;[|subst h;eapply path_front in Hπ; subst q; destruct π;cbn;eauto].
+    destruct Hq2;[contradiction|]. clear - H1. destruct π; cbn in *; eauto.
+  Qed.
+
+  Lemma minus_back_edge `{redCFG} edge' p q
+    : ((edge ∩ edge') ∖ (a_edge ∩ edge')) p q = true -> p ↪ q.
+  Proof.
+    intros Q.
+    unfold minus_edge,intersection_edge in Q. rewrite negb_andb in Q. conv_bool.
+    unfold back_edge,back_edge_b.
+    destruct Q as [[Q1 Q2] Q34]. unfold minus_edge. rewrite Q1; cbn. destruct Q34; eauto.
+    rewrite Q2 in H0; cbn in H0; congruence.
+  Qed.
+
+  Lemma loop_head_in_graph `{redCFG} h : loop_head h -> in_graph h.
+    intro Q.
+    unfold loop_head, in_graph in *. destruct Q as [q Q]. eapply minus_subgraph in Q. firstorder.
+  Qed.
+
+  Lemma dom_path `{redCFG} p q
+    : in_graph q -> Dom edge root p q -> p -->* q.
+  Proof.
+    intros Hin Hdom.
+    eapply reachability in Hin as [π Hπ]. specialize (Hdom π Hπ).
+    eapply path_from_elem in Hπ; eauto using Lab_dec. firstorder.
+  Qed.
+
+  Lemma loop_contains_not_dom `{redCFG} h q 
+    : loop_contains h q -> h <> q -> exists p, p ↪ h /\ ~ Dom edge q h p.
+  Proof.
+    intros Hloop Hneq. unfold loop_contains in Hloop. destructH.
+    unfold Dom; eexists; firstorder; eauto.
+    intros H0. destruct Hloop3;[|subst q;contradiction]. apply H1,H0. eauto.
+  Qed.
+
+  Lemma DM_not_exists X (p : X -> Prop) :
+    ~ (exists x, p x) <-> forall x, ~ p x.
+  Proof.
+    firstorder.
+  Qed.
+
+  Lemma not_and_iff (A B : Prop) : decidable A -> (~ (A /\ B) <-> ~ A \/ ~ B).
+  Proof.
+    firstorder.
+  Qed.
+
+  Lemma in_tl_in {A : Type} (a : A) (l : list A) : a ∈ tl l -> a ∈ l.
+  Proof.
+    destruct l; cbn in *; eauto.
+  Qed.
+
+  Lemma dom_loop_contains `{redCFG} h p q
+    : loop_contains h q -> ~ loop_contains h p -> Dom edge p h q.
+  Proof.
+    intros Hloop Hnloop.
+    decide' (p == q); [contradiction|].
+    unfold loop_contains in Hloop. destructH.
+    destruct Hloop3 as [Hloop3|Hloop3];[|subst q;eapply dominant_self]. rename π into π1.
+    intros π Hπ.
+    assert (in_graph p).
+    {
+      clear - Hπ c.
+      revert dependent q.
+      induction π; intros q c Hπ.
+      - inversion Hπ; contradiction.
+      - inversion_clear Hπ.
+        decide' (p == b).
+        + eexists. left; eauto.
+        + eapply IHπ;eauto.
+    }
+    eapply reachability in H0. destructH.
+    unfold loop_contains in Hnloop.
+    rewrite DM_not_exists in Hnloop. setoid_rewrite DM_not_exists in Hnloop.
+    eapply path_app in Hloop2;eauto.
+    specialize (Hnloop p0 (π1 :+ tl π)).
+    setoid_rewrite not_and_iff in Hnloop; [setoid_rewrite not_and_iff in Hnloop|].
+    - destruct Hnloop as [Hnloop|Hnloop]; [contradiction|destruct Hnloop].
+      + contradiction.
+      + clear - Hloop3 H1. eapply not_or in H1. destructH. eapply not_not in H0.
+        * eapply in_nl_conc in H0. destruct H0;[contradiction|]. eapply in_tl_in;eauto.
+        * eapply In_dec.
+    - edestruct path_dec;eauto; firstorder.
+    - edestruct (back_edge_dec p0 h); firstorder.
+      Unshelve. all:eauto.
+  Qed.
+
+  Lemma loop_contains_self `{redCFG} h : loop_head h -> loop_contains h h.
+  Proof.
+    intros Hl. unfold loop_contains.
+    - unfold loop_head in Hl. destruct Hl. 
+      eapply loop_head_dom in H0 as Hdom.
+      eapply back_edge_incl in H0 as Hreach. specialize (reachability x) as Hreach'.
+      exploit' Hreach'.
+      + eexists. left; apply Hreach.
+      + destructH.
+        eapply Hdom in Hreach' as Hreach''. eapply path_from_elem in Hreach'; eauto.
+        destructH; eauto. eexists; eexists. firstorder; eauto.
+  Qed.
+          
+  Lemma NoDup_rcons (A : Type) (x : A) (l : list A)
+    : x ∉ l -> NoDup l -> NoDup (l :r: x).
+  Proof.
+    intros Hnin Hnd. revert x Hnin.
+    induction Hnd; intros y Hnin; cbn.
+    - econstructor; eauto. econstructor.
+    - econstructor.
+      + rewrite in_app_iff. contradict Hnin. destruct Hnin; [contradiction|firstorder].
+      + eapply IHHnd. contradict Hnin. right; assumption.
+  Qed.
+
+  Lemma NoDup_nin_rcons (A : Type) (x : A) (l : list A)
+    : NoDup (l :r: x) -> x ∉ l.
+  Proof.
+    intros Hnd Hin.
+    dependent induction l.
+    - destruct Hin.
+    - destruct Hin; rewrite cons_rcons_assoc in Hnd; inversion Hnd.
+      + subst a. eapply H2. apply In_rcons;firstorder.
+      + eapply IHl; eauto.
+  Qed.
+  
+  Lemma loop_contains_path `{redCFG} h q π
+    : CPath h q π -> loop_contains h q -> NoDup π -> forall p, p ∈ π -> loop_contains h p.
+  Proof.
+    intros Hπ Hin Hnd p Hp. 
+    destruct (p == h) as [Hph|Hph].
+    - rewrite Hph. eapply loop_contains_self. eapply loop_contains_loop_head; eauto.
+    - destruct (loop_contains_dec h p) as [N|N]; [eauto|exfalso].
+      eapply path_from_elem in Hp; eauto. destructH.
+      eapply dom_loop_contains in N; eauto; cycle 1.
+      eapply postfix_incl in Hp1 as Hp1'; eauto.
+      dependent induction Hp1.
+      + eapply ne_to_list_inj in x. subst ϕ.
+        eapply Hph. eapply path_back in Hp0; eapply path_back in Hπ. rewrite <-Hp0. eauto.
+      + clear IHHp1. unfold Dom in N.
+        eapply postfix_incl in Hp1; eapply Hp1 in N; eauto.
+        rewrite rcons_nl_rcons in x. eapply ne_to_list_inj in x. rewrite <-x in Hnd.
+        eapply f_equal with (f:=ne_back) in x. simpl_nl' x. eapply path_back in Hπ. rewrite Hπ in x.
+        subst a.
+        eapply NoDup_nin_rcons; eauto. rewrite rcons_nl_rcons. assumption.
+  Qed.
+
+  Definition loop_edge `{redCFG} h := (fun q _ : Lab => loop_contains_b h q).
+
+  Lemma path_loop_edge `{redCFG} h q π
+    : CPath h q π -> (forall p, p ∈ π (* /\ p=q *) -> loop_contains h p)
+      -> Path (edge ∩ loop_edge h) h q π.
+  Proof.
+  Admitted.
+
+  Lemma loop_contains_ledge_head `{redCFG} h h' p
+    : loop_contains h p -> p ↪ h' -> loop_contains h h'.
+  Proof.
+  Admitted.
+
+  Program Instance loop_CFG
+          `(C : redCFG edge root a_edge)
+          (h : Lab)
+          (H : loop_head h)
+    : redCFG (edge ∩ loop_edge h)
+             h
+             (a_edge ∩ loop_edge h).
   Next Obligation.
-   Unset Printing Notations. 
+    eapply dom_intersection.
+    eapply dom_trans ; eauto.
+    - eapply reachability. eapply loop_head_in_graph in H; eapply H.
+    - eapply dom_loop;eauto. 
+      eapply loop_contains_ledge_head.
+      + eapply minus_subgraph in H0. eapply intersection_subgraph2 in H0.
+        unfold loop_edge,loop_contains_b in H0;eauto.
+        destruct loop_contains_dec; cbn in *;eauto;congruence.
+      + eapply minus_back_edge;eauto. 
+    - eapply loop_head_dom. eapply minus_back_edge; eauto.
+  Qed.
+  Next Obligation.
+    eapply intersection2_subgraph; apply a_edge_incl.
+  Qed.
+  Next Obligation.
+    eapply acyclic_subgraph_acyclic.
+    - eapply intersection_subgraph1.
+    - eapply a_edge_acyclic.
+  Qed.
 
-  Fixpoint implode' (G : redCFG) (l : list Lab) {struct l} : redCFG * (Lab -> option redCFG)
-    := .
-    
-   loop_depth, loop_head
+  Lemma loop_edge_reach_help `{redCFG} h p q
+        (Hhead : loop_head h)
+        (Hedge : (edge ∩ loop_edge h) p q = true)
+    : exists π, Path (edge ∩ loop_edge h) h p π.
+  Proof. 
+    enough (in_graph p) as Hin.
+    - enough (loop_contains h p) as Hcont.
+      + eapply dom_path with (p0:=h) in Hin as [π Hπ];[|eapply dom_loop;eauto].
+        specialize (path_NoDup _ _ _ _ _ (ex_intro _ π Hπ)) as [φ [Hφ Hnd]].
+        exists φ. eapply path_loop_edge;eauto. eapply loop_contains_path; eauto.
+      + unfold loop_edge in *; eapply intersection_subgraph2 in Hedge. unfold loop_contains_b in *.
+        edestruct loop_contains_dec;cbn in *;[eauto|congruence].
+    - eapply intersection_subgraph1 in Hedge; unfold in_graph;eexists;left;eauto.
+  Qed.
+  
+  Next Obligation.
+    destruct H1;[eapply loop_edge_reach_help;eauto|].
+    eapply loop_edge_reach_help in H1 as H1';eauto.
+    destructH. exists (q :<: π). econstructor; eauto.
+  Qed.
 
-  Parameter root_no_pred0 : forall p, p ∉ preds0 root.
+  Definition top_level `{redCFG} q := forall h, loop_contains h q -> (h = root \/ h = q).
+
+  (*  adding the  exit to the head is still missing *)
+
+  Parameter exit_edge_dec : forall `{redCFG} h q p, 
+      {exit_edge h p q} + {~ exit_edge h p q}.
+
+  Definition head_exits_edge `{redCFG} :=
+    ((fun p _ => p <>b root) ∩
+                         (fun h q
+                          => to_bool (Exists_dec (fun p => exit_edge h p q)
+                                                all_lab
+                                                (exit_edge_dec h q)))).
+
+  Program Instance head_exits_CFG `(C : redCFG edge root a_edge)
+    : redCFG (edge ∪ head_exits_edge) root (a_edge ∪ head_exits_edge).
+  Next Obligation.
+  Admitted.
+  Next Obligation.
+    eapply union_subgraph.
+    - exact a_edge_incl.
+    - firstorder.
+  Qed.
+  Next Obligation.
+  Admitted.
+  Next Obligation.
+  Admitted.
+
+  Definition implode_edge `{redCFG} := (fun p q => deq_loop_b root p && deq_loop_b root q).
+  
+  Program Instance implode_CFG `(C : redCFG edge root a_edge)
+    : redCFG (edge ∩ implode_edge) root (a_edge ∩ implode_edge).
+  Next Obligation.
+    eapply dom_intersection,loop_head_dom. eapply minus_back_edge; eauto.
+  Qed.
+  Next Obligation.
+    eapply intersection2_subgraph, a_edge_incl.
+  Qed.
+  Next Obligation.
+    eapply acyclic_subgraph_acyclic.
+    - eapply intersection_subgraph1.
+    - eapply a_edge_acyclic.
+  Qed.
+  Next Obligation.
+    specialize (@reachability _ _ _ C) as Hreach. unfold in_graph.
+  Admitted.
+
+  Definition local_impl_CFG `(C : redCFG) (h : Lab) (H : loop_head h) :=
+    implode_CFG (head_exits_CFG (loop_CFG C h H)).
+
+(*  Parameter root_no_pred0 : forall p, p ∉ preds0 root.*)
                  
   Parameter root : Lab.
   
-  Notation "p --> q" := (p ∈ preds0 q) (at level 55, right associativity).
+(*  Notation "p --> q" := (p ∈ preds0 q) (at level 55, right associativity).*)
   
   
   (** more parameters **)
-  Parameter all_lab : set Lab.
-  Parameter all_lab_spec : forall l, set_In l all_lab.
-  Notation "p -->? q" := (p === q \/ p --> q) (at level 70, right associativity).
-  Parameter loop_exit : forall `{Graph Lab}, Lab -> list Lab.
-  Parameter back_edge : Lab -> Lab -> Prop.
-  Parameter back_edge_dec : forall p q, {back_edge p q} + {~ back_edge p q}.
-  Parameter back_edge_incl : forall p q, back_edge p q -> p --> q.
   
   Lemma Lab_dec' : forall (l l' : Lab), { l = l' } + { l <> l'}.
   Proof.
     apply Lab_dec.
   Qed.
 
-  Definition is_back_edge (p q : Lab) :=
-    match (back_edge_dec p q) with | left _ => true | right _ => false end.
-  
-  Notation "p '-->*' q" := (exists π, Path p q π) (at level 70, right associativity).
+  Parameter no_self_loops : forall `(C : redCFG), forall q p, q --> p -> q =/= p.
 
-  Notation "p '-a>' q" := (In p (preds q) /\ ~ back_edge p q) (at level 70).
-  
-
-  Program Instance back_edge_CFG : Graph Lab root back_edge.
-  Next Obligation. apply back_edge_dec. Qed.
-  Next Obligation. intro H. eapply root_no_pred'. eapply back_edge_incl; eauto. Qed.
-
-  Definition acyclic_CFG := minus_Graph CFG back_edge_CFG.
-  
-  
-  Parameter loop_head_dec : forall p, {loop_head p} + {~ loop_head p}.
-
-  (** Paths **)
-      
-  Lemma acyclic_edge_has_edge : forall p q, p -a> q -> p --> q.
-  Proof.
-    intros. firstorder. 
-  Qed.
-
-  Definition acyclic_edge := (fun p q : Lab => cfg_edge p q /\ ~ back_edge p q).
-
-  Definition AcyPath : Lab -> Lab -> ne_list Lab -> Prop := @Path _ _ acyclic_edge _. 
-
-  Notation "p '-a>*' q" := (exists π, AcyPath p q π) (at level 70).
-  
-  (** Reducibility **)
-  Parameter reach_acy : forall (p : Lab), root -a>* p.
-  
-  Parameter loop_head_dom : forall ql qh, is_back_edge ql qh = true -> Dom qh ql.
-
-  
-  Parameter loop_exit_spec : forall qh qe,
-      In qh (loop_exit qe) <-> exists q, q --> qe /\ in_loop q qh /\ ~ in_loop qe qh.
-
-  Parameter no_self_loops :
-    forall q p, q --> p -> q =/= p.
-
-  Definition CPath := @Path _ _ _ CFG.
-
-  Definition CPath' `{Graph} π := CPath (ne_front π) (ne_back π) π.
-
-  (** collapsed CFG **)
-
-  Parameter depth : Lab -> nat.
-  Parameter depth_spec : True. (* TODO *)
-
-(*  Definition collapse_head (qh : Lab) := forall qe, qh ∈ exit qe -> 
-
-  Program Instance collapsed_CFG (col_dep : nat) : Graph Lab root (fun p q : Lab => if )*)
   
 End CFG.
-
-Import CFG.
 
 
 Module TCFG.
@@ -337,46 +903,37 @@ Module TCFG.
     | [ |- context[let (_,_) := ?a in _]] => destruct a
     end.
 
-  Program Instance TCFG (tag : Lab -> Lab -> Tag -> Tag) :
-    Graph Coord start_coord (fun c c'
-                             => let (p,i) := c  in
-                               let (q,j) := c' in
-                               cfg_edge p q /\ tag p q i = j
-                            ).
-  Next Obligation.
-    repeat destr_let. edestruct (@edge_dec _ _ _ CFG l l0); decide' (Tag_dec (tag l l0 t) t0);
-                        firstorder.
-  Qed.
-  Next Obligation.
-    repeat destr_let. intros [H H']. apply root_no_pred' in H. eauto.
-  Qed.
+  Definition tcfg_edge (edge : Lab -> Lab -> bool) (tag : Lab -> Lab -> Tag -> Tag) :=
+    (fun c c' : Coord => let (p,i) := c  in
+              let (q,j) := c' in
+              edge p q && (to_bool (Tag_dec (tag p q i) j))).
 
-  Fixpoint eff_tag p q i : Tag
-    := if is_back_edge p q
+  Fixpoint eff_tag `{redCFG} p q i : Tag
+    := if back_edge_b p q
        then match i with
             | nil => nil
             | n :: l => (S n) :: l
             end
        else 
-         let l' := @iter Tag (@tl nat) i (length (loop_exit p)) in
+         let l' := @iter Tag (@tl nat) i (exit_edge_num p q) in
          if loop_head_dec q then O :: l' else l'.
 
-  Definition TPath := @Path _ _ _ (TCFG eff_tag).
+  Definition TPath `{redCFG} := Path (tcfg_edge edge eff_tag).
 
-  Lemma TPath_CPath c c' π :
+  Lemma TPath_CPath `{redCFG} c c' π :
     TPath c c' π -> CPath (fst c) (fst c') (ne_map fst π).
   Proof.
-    intros H. dependent induction H; [|destruct b,c]; econstructor; cbn in *.
-    - apply IHPath.
-    - apply H0.
+    intros Q. dependent induction Q; [|destruct b,c]; econstructor; cbn in *.
+    - apply IHQ. 
+    - conv_bool. firstorder. 
   Qed.            
   
-  Definition TPath' `{Graph} π := TPath (ne_front π) (ne_back π) π.
+  Definition TPath' `{redCFG} π := TPath (ne_front π) (ne_back π) π.
   
-  Parameter eff_tag_fresh : forall p q q0 i j j0 l,
+  Parameter eff_tag_fresh : forall `{redCFG} p q q0 i j j0 l,
       TPath (q0,j0) (q,j) l -> eff_tag q p j = i -> forall i', In (p, i') l -> i' <> i.
 
-  Parameter eff_tag_det : forall q j p i i',
+  Parameter eff_tag_det : forall `{redCFG} q j p i i',
       eff_tag q p j = i ->
       eff_tag q p j = i' ->
       i = i'.
