Util.v
@@ -58,6 +58,18 @@ Proof.
   unfold nequiv_decb, equiv_decb. rewrite negb_false_iff. destruct (a == b); firstorder.
 Qed.
 
+Definition to_bool {P Q : Prop} (x : {P} + {Q}) := if x then true else false.
+
+Lemma to_bool_true (P : Prop) (x : {P} + {~ P}) : to_bool x = true <-> P.
+Proof.
+  destruct x; cbn; firstorder.
+Qed.
+    
+Lemma to_bool_false (P : Prop) (x : {P} + {~P}) : to_bool x = false <-> ~ P.
+Proof. 
+  destruct x; cbn; firstorder.
+Qed.
+
 Ltac conv_bool := repeat match goal with
                          | [ H: context[_ ==b _ = true] |- _ ] => rewrite beq_true in H
                          | [ H: context[_ ==b _ = false] |- _ ] => rewrite beq_false in H
@@ -67,6 +79,18 @@ Ltac conv_bool := repeat match goal with
                          | [ H: context[_ || _ = false] |- _ ] => rewrite orb_false_iff in H
                          | [ H: context[_ && _ = true] |- _ ] => rewrite andb_true_iff in H
                          | [ H: context[_ && _ = false] |- _ ] => rewrite andb_false_iff in H
+                         | [ H: context[to_bool _ = true] |- _ ] => rewrite to_bool_true in H
+                         | [ H: context[to_bool _ = false] |- _ ] => rewrite to_bool_false in H
+                         | [ |- context[_ ==b _ = true]] => rewrite beq_true
+                         | [ |- context[_ ==b _ = false]] => rewrite beq_false
+                         | [ |- context[_ <>b _ = true]] => rewrite bne_true
+                         | [ |- context[_ <>b _ = false]] => rewrite bne_false
+                         | [ |- context[_ || _ = true]] => rewrite orb_true_iff
+                         | [ |- context[_ || _ = false]] => rewrite orb_false_iff
+                         | [ |- context[_ && _ = true]] => rewrite andb_true_iff
+                         | [ |- context[_ && _ = false]] => rewrite andb_false_iff
+                         | [ |- context[to_bool _ = true]] => rewrite to_bool_true
+                         | [ |- context[to_bool _ = false]] => rewrite to_bool_false
                          end.
 
 Instance : forall A, EqDec A _ -> EqDec (option A) _ :=
